\documentclass[10pt,a4paper]{article}                            
\usepackage[utf8]{inputenc}                            
\usepackage[T1]{fontenc}                              
\usepackage{amsmath}                            
\usepackage{amsfonts}                            
\usepackage{amssymb}                            
\begin{document}
\setlength\parindent{0pt}
\subsection*{KKT conditions for constrained problem}

\textbf{Problem:}
\begin{flalign*}
\min_{x} & \, f\left( x\right)   \\
\text{subject to } & c_{E}\left( x\right) =0 \\
& c_{I}\left( x\right) -s=0 \\
& s\geq 0
\end{flalign*}\\\\


\textbf{Log-barrier method  problem with slack variables $S$:}
\begin{flalign*}
\min_{x,s} & \, f\left( x\right) -\lambda \sum ^{m}_{i=1}\log s_{i} \\
& c_{E}\left( x\right) =0 \\
& c_{I}\left( x\right) -s=0
\end{flalign*}
Note: $s_i > 0$ is satisfied automatically due to logarithm. \\\\

\textbf{Perturbed KKT conditions for log-barrier:}
\begin{flalign*}
&\nabla f\left( x\right) -A^{T}_{E}\left( x\right) y-A^{T}_{I}\left( x\right) z=0 \\
&-\lambda S^{-1}e+z=0 \text{ or } -\lambda e+ Sz=0\\ 
&c_{E}\left( x\right) =0 \\
&c_{I}\left( x\right) -s=0 \\
\end{flalign*}
Note:  $\lambda  e =  - Sz$

\noindent\makebox[\linewidth]{\rule{\paperwidth}{0.4pt}}

\textbf{My problem:}
\begin{flalign*}
 \min_{\tau} & \iint -sgn\left( v \right) u \,f_{Y}\left( u,v ;\tau \right) \,du\,dv \\
\text{subject to } & \kappa - \iint \text{sgn}\left( v \right) w\,f_{Z}\left( w,v;\tau \right)\, dw\,dv \geq 0 
\end{flalign*}\\


\textbf{Log-barrier formation:}
\begin{flalign*}
\min_{\tau ,s} &\iint -sgn\left( \nu \right) uf_{Y}\left( u,\nu ;\tau \right) \,du\,dv -\lambda \log s_{1} \\
\text{subject to } & \kappa  - \iint \text{sgn}\left( \nu \right) wf_{z}\left( w,v ;\tau \right) \,dw\,dv -s_{1}=0 
\end{flalign*}

Note: $s_1 > 0$ is satisfied automatically due to logarithm again. \\

\textbf{Perturbed KKT conditions:} \\

$ \exists \lambda ,z_{1},s_{1}$,   such that
\begin{gather*}
 \iint -sgn\left( \nu \right) u\nabla_{\tau} f_{Y}\left( u,\nu ;\tau \right) dud\nu -z_{1}\left\{ \kappa - \iint sgn\left( \nu \right) \omega \nabla _{\tau }f_{Z}\left( \omega ,\nu ;\tau \right) dwd\nu\right\} =0 \\
\kappa -\iint sgn\left( \nu \right) w\nabla _{\tau }f_{Z}\left( \omega ,\nu ;\tau \right) dwd\nu -s_{1}=0\\
-\lambda /s_{1}+z_{1}=0
\end{gather*}
From the last equation, we have $s_1 = \lambda / z_1 > 0$



\end{document}