\documentclass[12pt]{article}     
\usepackage[utf8]{inputenc}
\usepackage[english]{babel}
\usepackage{graphicx}
\graphicspath{{images/}{../images/}}
\usepackage{subfiles}
\usepackage{blindtext}
\newcommand{\pard[1]}{\frac{\partial}{\partial{#1}}}
\newcommand{\mean[1]}{\frac{1}{n}\sum_{i=1}^{#1}}
\newcommand{\defeq}{\vcentcolon=}
\newcommand{\eqdef}{=\vcentcolon}
\newcommand\independent{\protect\mathpalette{\protect\independenT}{\perp}}
\newcommand{\wh}{\widehat}
\newcommand{\itl}{\intercal}
\newcommand{\bs}{\boldsymbol}
\newcommand{\mb}{\mathbb}
\newcommand{\txt}{\text}
\newcommand{\lt}{\left}
\newcommand{\rt}{\right}
\newcommand{\nlim}{\underset{n \to \infty}{\lim}}
\newcommand{\smb}{\begin{bmatrix}}
\newcommand{\sme}{\end{bmatrix}}
\newcommand\indep{\protect\mathpalette{\protect\independenT}{\perp}}
\def\independenT#1#2{\mathrel{\rlap{$#1#2$}\mkern2mu{#1#2}}}
\newcommand{\tsgn}{\txt{sgn}}
\newcommand{\mnote}{\marginnote}
\def\independenT#1#2{\mathrel{\rlap{$#1#2$}\mkern2mu{#1#2}}}
\usepackage{amsmath}
\usepackage{graphicx}
\usepackage{verbatim}
%\usepackage{bbm}
%\usepackage{xfrac}
%\usepackage{dsfont}
\usepackage{amssymb}
\usepackage{verbatim}
\usepackage{mathtools}
\usepackage{resizegather}
\usepackage{xfrac}
\usepackage{amsthm}
\usepackage{mathrsfs}
\newtheorem{remark}{Remark}
\newtheorem{lemma}{Lemma}
\newtheorem{theorem}{Theorem}
\newtheorem{corollary}{Corollary}
\renewcommand\qedsymbol{$\blacksquare$}
\usepackage{setspace}
\doublespacing
%\theoremstyle{definition}
%\newtheorem{definition}{Definition}[section]
%\theoremstyle{remark}
%\newtheorem*{remark}{Remark}
%\newtheorem{theorem}{Theorem}[section]
%\newtheorem{corollary}{Corollary}[theorem]
%\newtheorem{lemma}[theorem]{Lemma}
\usepackage[a4paper, total={7.4in, 9.6in}]{geometry}   
\usepackage[backend=bibtex,style=numeric]{biblatex}
\addbibresource{main.bib} 
\title{Two Stage Treatment Regime Draft Asymptotics of $\bs{\tau}}
\begin{document}
Before we derive the limiting distribution of the estimator $\hat{\bs{\tau}}_{\kappa,\mu}$, we need to examine, for any fixed value of $\bs{\tau}: \bs{\tau}_1^\itl\bs{\tau}_1 = 1$ and $\bs{\tau}_2^\itl\bs{\tau}_2 = 1$, the limiting distribution of $\nabla \wh{\mb{E}} Y_n(\bs{\tau})$.
\begin{flalign*}
\nabla \wh{\mb{E}} Y_n(\bs{\tau}) = &\pard[\bs{\tau}] \int y \,d \wh{F}_{Y_n(\bs{\tau})}(y) \\
= &\pard[\bs{\tau}] \int y \,d \lt[ \mean[n] \wh{F}_{Y_n(\bs{\tau})}(y | \bs{H}_{1,i} = \bs{h}_{1,i}) \rt] \\
= & \mean[n] \pard[\bs{\tau}] \int y \,d  \wh{F}_{Y_n(\bs{\tau})}(y | \bs{H}_{1,i} = \bs{h}_{1,i})  \\
%= &  \nabla\int y \lt[ \,d \iint  F_{\epsilon}\lt\{ y - m_Y - \tsgn(r_2)c_Y\rt\}\,d G_{Y}\lt\{ m_Y, c_Y, r_2 \mid \bs{h}_1 , d_1(\bs{h}_1)\rt\} \,d F_{\bs{H}_1}(\bs{h}_1) \rt] \\
%= &  \nabla\int y \lt[ \,d \iint  F_{\epsilon}\lt\{ y - m_Y - \tsgn(r_2)c_Y\rt\}\,d G_{Y}\lt\{ m_Y, c_Y, r_2 \mid \bs{h}_1 , d_1(\bs{h}_1)\rt\} \,d F_{\bs{H}_1}(\bs{h}_1) \rt] 
\end{flalign*}
%\begin{gather}
%\begin{flalign*}
%\nabla_{\bs{\tau}}\wh{\mathbb{E}}\lt\{ \text{sgn}\lt(\bs{X}^{\intercal}\bs{\tau}\rt)\bs{X}_1^{\intercal}\bs{\beta}_{Y1}\rt\} =\nabla_{\bs{\tau}}\lt[\frac{1}{n}\sum_{i=1}^{n}\bs{X}_{i,1}^{\intercal}\bs{\beta}_{Y1}\lt\{ 1-2K\lt(-\frac{\bs{X}^{\intercal}_{i}\bs{\tau}}{h}\rt)\rt\} \rt]=\frac{1}{n}\sum_{i=1}^{n}\frac{2\bs{X}_{i,1}^{\intercal}\bs{\beta}_{Y1}}{h}k\lt(-\frac{\bs{X}_{i}^{\intercal}\bs{\tau}}{h}\rt)\bs{X}_{i}.
%\end{flalign*}
%\end{gather}

\begin{lemma}
In addition to the assumptions in corollary 1, we also suppose the following conditions hold.
\begin{enumerate}
\item $\bs{X}^{\intercal}\bs{\tau}$ is bounded away from 0.
\item $\forall \bs{a} \in \mathbb{R}^p$,$\exists \delta > 0$ ,such that 
\begin{enumerate}
\item $\mathbb{E}\lt|\bs{a}^\itl\pard[\bs{\tau}] \int y \,d  \wh{F}_{Y_n(\bs{\tau})}(y | \bs{H}_{1,i} = \bs{h}_{1,i})\rt|^{2+\delta} < \infty$ 
\item $ \lt\{\bs{\bs{a}^{\intercal}}V\lt[\pard[\bs{\tau}] \int y \,d  \wh{F}_{Y_n(\bs{\tau})}(y | \bs{H}_{1,i} = \bs{h}_{1,i})\rt]\bs{a} \rt\}^{1+\frac{\delta}{2}}< \infty$.
\end{enumerate}
\end{enumerate} 
Then, we have, for any fixed $\bs{\tau}$ and $\bs{\beta}_{Y1}$,
\begin{gather}
\begin{flalign*}
\sqrt{n}\lt[\nabla \wh{\mb{E}} Y_n(\bs{\tau})  -\mathbb{E}\lt(\nabla \wh{\mb{E}} Y_n(\bs{\tau})\rt)\rt]\overset{d}{\to}N\lt(0,AV\lt[\pard[\bs{\tau}] \int y \,d  \wh{F}_{Y_n(\bs{\tau})}(y | \bs{H}_{1,i} = \bs{h}_{1,i}) \rt]\rt)
\end{flalign*}
\end{gather}
\end{lemma}

The proof of this is similar to the proof of Lemma 1 in the one-stage problem.
%\subsection{Limiting distribution of $\nabla_{\bs{\tau}}\wh{\mathbb{E}}\lt\{ \text{sgn}\lt(\bs{X}^{\intercal}\bs{\tau}\rt)\bs{X}_1^{\intercal}\bs{\beta}_{Y1}\rt\} $}

%Comment: Goal is to prove the derivative above is asymptotically normal.
%Considering that it includes sample size $n$ in $h$, and it is multivariate.
%Try Lyapunov condition and cramer-wold theorem first.
%
%The sequences here are a triangular array, and are iid for each $n$.
%
%$k$ is the kernel of our choice, gaussian kernel.

\begin{proof}
For any  $\bs{a} \in \mathbb{R}^p$, we let $W_{ni} = \bs{a}^\itl \pard[\bs{\tau}]\int y \,d  \wh{F}_{Y_n(\bs{\tau})}(y | \bs{H}_{1,i} = \bs{h}_{1,i})$. For each value of $n$, $w_{n1},w_{n2},\cdots,w_{nn}$ are i.i.d, and functions of the sample size $n$. This is because that $\bs{X}_{i}$ are assumed to be i.i.d., and $h$ is a function of sample
size $n$. Then, we have
\begin{gather*}
\mu_{n}:=\mathbb{E}W_{ni}=\mathbb{E}\lt[\bs{a}^\itl \pard[\bs{\tau}]\int y \,d  \wh{F}_{Y_n(\bs{\tau})}(y | \bs{H}_{1,i} = \bs{h}_{1,i})\rt],
\end{gather*}
and 
\begin{gather*}
\sigma_{n}^{2}:=V(W_{ni})=\bs{a}^\itl V\lt[\pard[\bs{\tau}]\int y \,d  \wh{F}_{Y_n(\bs{\tau})}(y | \bs{H}_{1,i} = \bs{h}_{1,i}) \rt]\bs{a}
\end{gather*}

%?????????????????????????????????????????????????????????? \\
%??? Delta method and Taylor expansion for approximation ??? \\
%?????????????????????????????????????????????????????????? \\
We let $G_{ni}=W_{ni}-\mu_{\ensuremath{n}}$, and $T_{n}=\sum_{i=1}^{n}G_{ni}$. Also, we let $s_{n}^{2}=V(T_{n})=\sum_{i=1}^{n}V(G_{ni})=\sum_{i=1}^{n}\sigma_{n}^{2}=n\sigma_{n}^{2}$, where the second equality is because of independence, and the last equality is due to identicalness. Therefore, $\sfrac{T_{n}}{s_{n}}$ has mean 0, and variance 1.  If we can show $G_{ni}$ satisfying the Lyapunov condition, then
we have

$\frac{T_{n}}{s_{n}}\overset{d}{\to}N(0,1)$,

as $n \to \infty$.

Now, we check the Lyapunov condition, that is,~\cite{Lindsay1995,Hunter2014}
\begin{gather*}
\exists\delta>0, \text{ such that } \frac{1}{s_{n}^{2+\delta}}\sum_{i=1}^{n}\mathbb{E}\mid G_{n,i}\mid^{2+\delta}\to0, \text{ as } n\to0. 
\end{gather*}
We define, for any $\bs{a}$, 
\begin{gather*}
C_1 \triangleq \mathbb{E}\lt|G_{ni}\rt|^{2+\delta}=\mathbb{E}\lt|W_{ni}-\mu_{\ensuremath{n}}\rt|^{2+\delta}=\mathbb{E}\lt|\bs{a}^\itl \pard[\bs{\tau}]\int y \,d  \wh{F}_{Y_n(\bs{\tau})}(y | \bs{H}_{1,i} = \bs{h}_{1,i})-\mu_{n}\rt|^{2+\delta},
\end{gather*}
and 
\begin{gather*}
C_2 \triangleq s_{n}^{2+\delta}=n^{1+\frac{\delta}{2}}\sigma_{n}^{2+\delta}=n^{1+\frac{\delta}{2}}\lt\{ \bs{a}^\itl  V \lt[ \pard[\bs{\tau}]\int y \,d  \wh{F}_{Y_n(\bs{\tau})}(y | \bs{H}_{1,i} = \bs{h}_{1,i}) \rt] \bs{a} \rt\} ^{1+\frac{\delta}{2}}.
\end{gather*}
Then, we have
\begin{flalign*}
&\frac{1}{s_{n}^{2+\delta}}\sum_{i=1}^{n}\mathbb{E}\mid G_{n,i}\mid^{2+\delta}\\
=&\frac{\mathbb{E}\lt|\bs{a}^\itl \pard[\bs{\tau}]\int y \,d  \wh{F}_{Y_n(\bs{\tau})}(y | \bs{H}_{1,i} = \bs{h}_{1,i})-\mu_{n}\rt|^{2+\delta}}{n^{\frac{\delta}{2}}\lt\{ \bs{a}^{\intercal}V\lt[\pard[\bs{\tau}]\int y \,d  \wh{F}_{Y_n(\bs{\tau})}\lt(y | \bs{H}_{1,i} = \bs{h}_{1,i}\rt) \rt]\bs{a}\rt\} ^{1+\frac{\delta}{2}}} \\
=&\frac{C_{1}}{n^{\frac{\delta}{2}}C_{2}}.
\end{flalign*}

As long as $\delta>0$, for finite $C_1$ and finite $C_2$, we have $\sfrac{C_{1}}{n^{\frac{\delta}{2}}C_{2}}\to0$,
as $n\to\infty$. This means that the Lyapunov condition is satisfied, if $\mathbb{E}\lt|G_{ni}\rt|^{2+\delta}$ and $s_{n}^{2+\delta}$ are finite. Then,  by Lyapunov Central Limit Theorem, we have
\begin{gather*}
\frac{T_{n}}{s_{n}}\overset{d}{\to}N(0,1).
\end{gather*}

As this hold for any arbitary non-random vector $\bs{a}\in \mathbb{R}^p$, we have, by Cramer-Wold Theorem, that
\begin{gather*}
\sqrt{n}\lt[\mean[n] \pard[\bs{\tau}]\int y \,d  \wh{F}_{Y_n(\bs{\tau})}(y | \bs{H}_{1,i} = \bs{h}_{1,i}) -\mathbb{E}\lt\{ \pard[\bs{\tau}]\int y \,d  \wh{F}_{Y_n(\bs{\tau})}(y | \bs{H}_{1,i} = \bs{h}_{1,i})\rt\}\rt]\overset{d}{\to}N\lt(0,V\lt[\pard[\bs{\tau}]\int y \,d  \wh{F}_{Y_n(\bs{\tau})}(y | \bs{H}_{1,i} = \bs{h}_{1,i})\rt]\rt),
\end{gather*}
as $n \to \infty$. We denote $\bs{L}_{ni}= \pard[\bs{\tau}]\int y \,d  \wh{F}_{Y_n(\bs{\tau})}(y | \bs{H}_{1,i} = \bs{h}_{1,i})$,
then this is written as
\begin{gather*}
\sqrt{n}\lt[\frac{1}{n}\sum_{i=1}^{n}\bs{L}_{ni}-\mathbb{E}\bs{L}_{n1}\rt]\overset{d}{\to}N\lt(0,V\lt[\bs{L}_{n1}\rt]\rt).
\end{gather*}
Then, we have
\begin{gather*}
\frac{1/n\sum_{i=1}^{n}\bs{L}_{ni}-\mathbb{E}\bs{L}_{n1}}{[V(\bs{L}_{n1})/n]^{1/2}}\frac{[V(\bs{L}_{n1})/n]^{1/2}}{\lt[AV(\bs{L}_{n1})/n\rt]^{1/2}}\overset{d}{\to}N(0,1).
\end{gather*}
As  $n \to \infty$, 
\begin{gather*}
\frac{V(\bs{L}_{n1})^{1/2}}{AV(\bs{L}_{n1})^{1/2}}\to1,
\end{gather*}
then we have
\begin{gather*}
\frac{1/n\sum_{i=1}^{n}\bs{L}_{ni}-\mathbb{E}\bs{L}_{n1}}{[AV(\bs{L}_{n1})/n]^{1/2}}\overset{d}{\to}N(0,1),
\end{gather*}
i.e.,
\begin{gather*}
\sqrt{n}\lt[1/n\sum_{i=1}^{n}\bs{L}_{ni}-\mathbb{E}\bs{L}_{n1}\rt]\overset{d}{\to}N\lt(0,AV(\bs{L}_{n1})\rt).
\end{gather*}
As $\frac{1}{n}\sum_{i=1}^{n}\bs{L}_{ni} =\mean[n] \pard[\bs{\tau}]\int y \,d  \wh{F}_{Y_n(\bs{\tau})}(y | \bs{H}_{1,i} = \bs{h}_{1,i}) = \nabla \wh{\mb{E}} Y_n(\bs{\tau})$, we have
\begin{gather}
\begin{flalign*}
\sqrt{n}\lt[\nabla \wh{\mb{E}} Y_n(\bs{\tau})  -\mathbb{E}\lt\{\nabla \wh{\mb{E}} Y_n(\bs{\tau})\rt\}\rt]\overset{d}{\to}N\lt(0,AV\lt[\pard[\bs{\tau}] \int y \,d  \wh{F}_{Y_n(\bs{\tau})}(y | \bs{H}_{1,i} = \bs{h}_{1,i}) \rt]\rt)
\end{flalign*}
\end{gather}
\end{proof}
Assume $\wh{F}_{Y_n(\bs{\tau})}(y | \bs{H}_{1,i} = \bs{h}_{1,i})$, the following lemma shows that the estimations do not effect the limiting distribution obtained above.
\begin{corollary}
Suppose all the assumptions in Lemma 3  hold, and $\wh{F}_{Y_n(\bs{\tau})}(y | \bs{H}_{1,i} = \bs{h}_{1,i})$ are consistent estimators of ${F}_{Y^*(\bs{\tau})}(y | \bs{H}_{1,i} = \bs{h}_{1,i})$. Then, we have
\begin{gather}
\begin{flalign*}
\sqrt{n}\lt[\nabla \wh{\mb{E}} Y_n(\bs{\tau})  - \nabla \mb{E}Y^*_n(\bs{\tau})\rt]\overset{d}{\to}N\lt(0,AV\lt[\pard[\bs{\tau}] \int y \,d  F_{Y^*(\bs{\tau})}(y | \bs{H}_{1,i} = \bs{h}_{1,i}) \rt]\rt)
\end{flalign*}
\end{gather}
\end{corollary}
\begin{proof}
We write
\begin{gather}
\begin{flalign*}
& \nabla \wh{\mb{E}} Y_n(\bs{\tau})  - \nabla \mb{E}Y^*(\bs{\tau}) \\
= & \nabla \wh{\mb{E}} Y_n(\bs{\tau})  - \mb{E}\lt\{ \nabla \wh{\mb{E}}Y_n(\bs{\tau}) \rt\}  + \mb{E}\lt\{ \nabla \wh{\mb{E}}Y_n(\bs{\tau}) \rt\}\ - \nabla \mb{E}Y^*(\bs{\tau}),
\end{flalign*}
\end{gather}
where $ \mb{E}\lt\{ \nabla \wh{\mb{E}}Y_n(\bs{\tau}) \rt\}\ - \nabla \mb{E}Y^*(\bs{\tau}) =  \mb{E}\lt\{\pard[\bs{\tau}]\int y \,d  \wh{F}_{Y_n(\bs{\tau})}(y | \bs{H}_{1,i} = \bs{h}_{1,i})\rt\}  - \mb{E} \pard[\bs{\tau}]\int y \,d  F_{Y^*x(\bs{\tau})}(y | \bs{H}_{1,i} = \bs{h}_{1,i}) = o_p(1)$ is due to the consistency of $\wh{F}_{Y_n(\bs{\tau})}(y | \bs{H}_{1,i} = \bs{h}_{1,i})$ and dominated convergence theorem.\\
By lemma 1, we have
\begin{gather}
\begin{flalign*}
\sqrt{n}\lt[\nabla \wh{\mb{E}} Y_n(\bs{\tau})  -\mathbb{E}\lt\{\nabla \wh{\mb{E}} Y_n(\bs{\tau})\rt\}\rt]\overset{d}{\to}N\lt(0,AV\lt[\pard[\bs{\tau}] \int y \,d  \wh{F}_{Y_n(\bs{\tau})}(y | \bs{H}_{1,i} = \bs{h}_{1,i}) \rt]\rt)
\end{flalign*}
\end{gather}

As $\wh{F}_{Y_n(\bs{\tau})}(y | \bs{H}_{1,i} = \bs{h}_{1,i})$ is consistent, we have
\begin{gather*}
\frac{AV\lt[\pard[\bs{\tau}] \int y \,d  \wh{F}_{Y_n(\bs{\tau})}(y | \bs{H}_{1,i} = \bs{h}_{1,i}) \rt]}{AV\lt[\pard[\bs{\tau}] \int y \,d  F_{Y^*(\bs{\tau})}(y | \bs{H}_{1,i} = \bs{h}_{1,i}) \rt]} \overset{p}{\to} 1.
\end{gather*}
Then, we have
\begin{gather}
\begin{flalign*}
\sqrt{n}\lt[\nabla \wh{\mb{E}} Y_n(\bs{\tau})  - \nabla \mb{E}Y^*(\bs{\tau})\rt]\overset{d}{\to}N\lt(0,AV\lt[\pard[\bs{\tau}] \int y \,d  F_{Y^*_n(\bs{\tau})}\lt(y | \bs{H}_{1,i} = \bs{h}_{1,i}\rt) \rt]\rt)
\end{flalign*}
\end{gather}
\end{proof}		


\textbf{Limiting distribution of $\wh{\bs{\tau}}_{\kappa,\mu}$}\\
Now, we investigate the limiting distribution of $\wh{\bs{\tau}}_{\kappa,\mu}$.

\begin{theorem}
Suppose all the assumptions above hold. Then we have, as $n\to \infty$
\begin{flalign*}
\sqrt{n}(\wh{\bs{\tau}}_{\kappa,\mu} - \bs{\tau}_{\kappa,\mu}^*) \overset{d}{\to} N\lt(\bs{0}, \bs{\Sigma}^* \rt),
\end{flalign*}
where $\bs{\Sigma}^* = \bs{D}^{*-1}\bs{C}^{*}\bs{D}^{*-1}$, 
\begin{flalign*}
\bs{C}^* :=
AV\lt[\pard[\bs{\tau}] \int y \,d F_{Y^*(\bs{\tau})}(y | \bs{H}_{1} = \bs{h}_{1}) \rt],
\end{flalign*}
and
\begin{gather*}                 
\begin{flalign*}
\bs{D}^*:= &\nabla^2 \mb{E} Y^*(\bs{\tau}^*_{\kappa,\mu}) - \mu \frac{\nabla^2 \mb{E} Z^*(\bs{\tau}^*_{\kappa,\mu}) \lt[ \kappa - \mb{E} Z^*(\bs{\tau}^*_{\kappa,\mu}) \rt] + \{ \nabla \mb{E} Z^*(\bs{\tau}^*_{\kappa,\mu}) \}^2}{  \lt\{\kappa - \mb{E} Z^*(\bs{\tau}^*_{\kappa,\mu}) \rt\}^2} \\
= & \nabla^2 {S}^* (\bs{\tau}_{\kappa,\mu}^*, \mu).
\end{flalign*}
\end{gather*}
with  $\bs{A}^{\prime}_0(\bs{\tau}^*_{\kappa, \mu}, \bs{\beta}^*_{Y1})= \mathbb{E} \{ 2\bs{X}_1^{\intercal}\bs{\beta}^*_{Y1}\delta\lt(\bs{X}^{\intercal}\bs{\tau}_{\kappa,\mu}^*\rt)\bs{X}\}$ and $\bs{A}_0^{\prime\prime}(\bs{\tau}_{\kappa,\mu}^*, \bs{\beta}_{Y1}^*) = \mathbb{E}\lt[ 2\bs{X}_1^{\intercal}\bs{\beta}^*_{Y1}\delta^{\prime}\lt(\bs{X}^{\intercal}\bs{\tau}_{\kappa,\mu}^*\rt)\bs{X}\bs{X}^{\intercal}\rt].$ 
\end{theorem}
\begin{proof}

Taylor expansion, for each $\mu$ 
$$\nabla\wh{S}(\bs{\tau}^*_{\kappa,\mu},\mu) = \nabla\wh{S}(\wh{\bs{\tau}}_{\kappa,\mu},\mu) - \nabla^2\wh{S}(\tilde{\bs{\tau}}_{\kappa,\mu}, \mu) (\wh{\bs{\tau}}_{\kappa,\mu} - \bs{\tau}^*_{\kappa,\mu} ),$$ 
where $\tilde{\bs{\tau}}_{\kappa,\mu}$ is a vector in between $\wh{\bs{\tau}}_{\kappa,\mu}$ and $\bs{\tau}^*_{\kappa,\mu}$.
As $\wh{\bs{\tau}}_{\kappa}(\mu)$ is the maximizer of $\wh{S}(\bs{\tau}, \mu)$, it satifies the first order condtion such that $\nabla\wh{S}(\wh{\bs{\tau}}_{\kappa,\mu},\mu) = 0$. Then,
\begin{flalign*}
& \sqrt{n}\nabla\wh{S}(\bs{\tau}^*_{\kappa,\mu},\mu) =  -\sqrt{n} \nabla^2\wh{S}(\tilde{\bs{\tau}}_{\kappa,\mu},\mu ) (\wh{\bs{\tau}}_{\kappa,\mu} - \bs{\tau}^*_{\kappa,\mu} )\\
& \nabla\wh{S}(\bs{\tau}^*_{\kappa,\mu},\mu) = \nabla \wh{\mb{E}} Y_n(\bs{\tau}^*_{\kappa,\mu}) - \mu \frac{\nabla \wh{\mb{E}} Z_n(\bs{\tau}^*_{\kappa,\mu})}{  \kappa - \wh{\mb{E}} Z_n(\bs{\tau}^*_{\kappa,\mu}) } + + \frac{2}{\mu}\,(\bs{\tau}_{\kappa,\mu}^{*\intercal}\bs{\tau}^*_{\kappa,\mu}-1)\bs{\tau}^*_{\kappa,\mu}, 
\txt{where }\bs{\tau}_{\kappa,\mu}^{*\itl}\bs{\tau}^*_{\kappa,\mu}-1 = 0.\\
& \nabla^2\wh{S}(\bs{\tau}^*_{\kappa,\mu}, \mu) = \nabla^2 \wh{\mb{E}} Y_n(\bs{\tau}^*_{\kappa,\mu}) - \mu \frac{\nabla^2 \wh{\mb{E}} Z_n(\bs{\tau}^*_{\kappa,\mu}) \lt[ \kappa - \wh{\mb{E}} Z_n(\bs{\tau}^*_{\kappa,\mu}) \rt] + \{ \nabla \wh{\mb{E}} Z_n(\bs{\tau}^*_{\kappa,\mu}) \}^2}{  \lt\{\kappa - \wh{\mb{E}} Z_n(\bs{\tau}^*_{\kappa,\mu}) \rt\}^2} 
\end{flalign*}
Then, we have 
\begin{flalign*}
\nabla\wh{S}(\bs{\tau}^*_{\kappa,\mu},\mu) = \nabla \wh{\mb{E}} Y_n(\bs{\tau}^*_{\kappa,\mu}) - \mu \frac{\nabla \wh{\mb{E}} Z_n(\bs{\tau}^*_{\kappa,\mu})}{  \kappa - \wh{\mb{E}} Z_n(\bs{\tau}^*_{\kappa,\mu}) },
\end{flalign*}

%As the left hand side is asymptotically normal with mean $\bs{0}$ and 
By Lemma 2 , we have  the first term on the right hand side as
\begin{gather}
\begin{flalign*}
\nabla \wh{\mb{E}} Y_n(\bs{\tau})  \overset{d}{\to}N\lt\{\nabla \mb{E}Y^*(\bs{\tau}),\frac{1}{n}AV\lt[\pard[\bs{\tau}] \int y \,d F_{Y^*(\bs{\tau})}(y | \bs{H}_{1} = \bs{h}_{1}) \rt]\rt\}
\end{flalign*}
\end{gather}
For the second term on the right hand side, we also have that 
\begin{gather*}
\mu \frac{\nabla \wh{\mb{E}} Z_n(\bs{\tau}^*_{\kappa,\mu})}{  \kappa - \wh{\mb{E}} Z_n(\bs{\tau}^*_{\kappa,\mu}) } \overset{p}{\to} \mu \frac{\nabla \mb{E} Z(\bs{\tau}^*_{\kappa,\mu})}{  \kappa - \mb{E} Z(\bs{\tau}^*_{\kappa,\mu}) },,
\end{gather*}
where we assume  both $\kappa - \wh{\mb{E}} Z_n(\bs{\tau}^*_{\kappa,\mu}) > 0$ and $\kappa - \mb{E} Z(\bs{\tau}^*_{\kappa,\mu}) > 0$ . This convergence in probablity is due to the consitency of $\wh{F}_{Z_n(\bs{\tau})}(z | \bs{H}_1 = \bs{h}_1)$ and dominated convergence theorem. Together, by Sluskty's theorem and the stationarity of $\bs{\tau}^*_{\kappa,\mu}$ of $S^*(\bs{\tau}, \mu)$, we have 
\begin{flalign*}
\sqrt{n} \nabla\wh{S}( {\bs{\tau}}^*_{\kappa,\mu}, \mu) \overset{d}{\to} N\lt(0, \bs{C}^*\rt),
\end{flalign*}
where 
\begin{flalign*}
\bs{C}^* :=
AV\lt[\pard[\bs{\tau}] \int y \,d F_{Y^*(\bs{\tau})}(y | \bs{H}_{1} = \bs{h}_{1}) \rt]
\end{flalign*}

We have that  $\nabla^2\wh{S}(\tilde{\bs{\tau}}_{\kappa,\mu}, \mu) = \nabla^2\wh{S}(\bs{\tau}^*_{\kappa,\mu}, \mu) + o_p(1)$,  as $\tilde{\bs{\tau}}_{\kappa,\mu}$ is in between $\wh{\bs{\tau}}_{\kappa,\mu}$ and $\bs{\tau}^*_{\kappa,\mu}$ and $\wh{\bs{\tau}}_{\kappa,\mu} - \bs{\tau}^*_{\kappa,\mu} = o_p(1)$. 
Therefore, we have            
\begin{flalign*}
\bs{D}^* \triangleq & p\underset{n \to \infty}{\lim}\nabla^2_{\bs{\tau}}\wh{S}_{\kappa} (\tilde{\bs{\tau}}_{\kappa, \mu}, \mu) \\
= & p\underset{n \to \infty}{\lim} \lt[\nabla^2 \wh{\mb{E}} Y_n(\bs{\tau}^*_{\kappa,\mu}) - \mu \frac{\nabla^2 \wh{\mb{E}} Z_n(\bs{\tau}^*_{\kappa,\mu}) \lt[ \kappa - \wh{\mb{E}} Z_n(\bs{\tau}^*_{\kappa,\mu}) \rt] + \{ \nabla \wh{\mb{E}} Z_n(\bs{\tau}^*_{\kappa,\mu}) \}^2}{  \lt\{\kappa - \wh{\mb{E}} Z_n(\bs{\tau}^*_{\kappa,\mu}) \rt\}^2}\rt] \\
= &\nabla^2 \mb{E} Y^*(\bs{\tau}^*_{\kappa,\mu}) - \mu \frac{\nabla^2 \mb{E} Z^*(\bs{\tau}^*_{\kappa,\mu}) \lt[ \kappa - \mb{E} Z^*(\bs{\tau}^*_{\kappa,\mu}) \rt] + \{ \nabla \mb{E} Z^*(\bs{\tau}^*_{\kappa,\mu}) \}^2}{  \lt\{\kappa - \mb{E} Z^*(\bs{\tau}^*_{\kappa,\mu}) \rt\}^2} \\
= & \nabla^2 {S}^* (\bs{\tau}_{\kappa,\mu}^*, \mu).
\end{flalign*}
\end{proof}
We can estimate $\bs{\Sigma}^*$ by plug in the corresponding estimators stated, and denote the estimator $\wh{\bs{\Sigma}}$, that is, $\wh{\bs{\Sigma}} = \wh{\bs{D}}^{-1}\wh{\bs{C}}\wh{\bs{D}}^{-1}$, 

\begin{flalign*}
\wh{\bs{C}} = & \wh{V}\lt\{\pard[\bs{\tau}] \int y \,d \wh{F}_{Y_n(\wh{\bs{\tau}}_{\kappa,\mu})}(y | \bs{H}_{1} = \bs{h}_{1}) \rt\} \\
= & \wh{V} \lt[\nabla \wh{\mb{E}} \lt\{Y_n(\wh{\bs{\tau}}_{\kappa,\mu}) \mid \bs{H}_1 =\bs{h_1}\rt\}\rt]
\end{flalign*}

and
\begin{gather*}                 
\begin{flalign*}
\wh{\bs{D}} =   \nabla^2\wh{S}(\wh{\bs{\tau}}_{\kappa,\mu}, \mu) = \nabla^2 \wh{\mb{E}} Y_n(\wh{\bs{\tau}}_{\kappa,\mu}) - \mu \frac{\nabla^2 \wh{\mb{E}} Z_n(\wh{\bs{\tau}}_{\kappa,\mu}) \lt[ \kappa - \wh{\mb{E}} Z_n(\wh{\bs{\tau}}_{\kappa,\mu}) \rt] + \{ \nabla \wh{\mb{E}} Z_n(\wh{\bs{\tau}}_{\kappa,\mu}) \}^2}{  \lt\{\kappa - \wh{\mb{E}} Z_n(\wh{\bs{\tau}}_{\kappa,\mu}) \rt\}^2},
\end{flalign*}
\end{gather*}

Step 1:  $\underset{\bs{\tau}:\bs{\tau}_1^\itl \bs{\tau}_1=1, \bs{\tau}_2^\itl \bs{\tau}_2=1}{\sup}\lt|\wh{S}_{\kappa}(\bs{\tau}, \mu)-S^*_{\kappa}(\bs{\tau},  \mu)\rt|=o_{p}(1).$ \\

Step 2:  conditions for $\wh{F}_{Y_n}(y;\bs{\tau}) \to F_Y(y;\bs{\tau}), \text{as } n \to \infty$\\

Step 3:  Consistency of $\wh{\bs{\tau}}_{\kappa,\mu} \to \bs{\tau}^*_{\kappa,\mu}$. It can be proven by following similar proof in Lemma 2 at one-stage. \\

Step 4: Asymptotic Normality of $\wh{\bs{\tau}}_{\kappa,\mu}$ \\

Step 5: Projected CI for $\wh{\mb{E}} Y_n(\wh{\bs{\tau}}_{n,\kappa})$\\

Step 6: Bootstrap Monte Carlo Sampling\\
\end{document}